Add a var cx

src/dynamics.lean
@@ -1,13 +1,20 @@
 import syntax
 
-inductive steps: exp -> exp -> Prop
+inductive vcx: Type
+| nil: vcx
+| cons: vcx -> var -> val -> vcx
+
+inductive steps: vcx -> exp -> exp -> Prop
 | if_e1
+    (Δ: vcx)
     (e1: exp) (e1': exp) (e2: exp) (e3: exp):
-    steps e1 e1' ->
-    steps (exp.if_ e1 e2 e3) (exp.if_ e1' e2 e3)
+    steps Δ e1 e1' ->
+    steps Δ (exp.if_ e1 e2 e3) (exp.if_ e1' e2 e3)
 | if_true
+    (Δ: vcx)
     (e2: exp) (e3: exp):
-    steps (exp.if_ (exp.pure val.true) e2 e3) e2
+    steps Δ (exp.if_ (exp.pure val.true) e2 e3) e2
 | if_false
+    (Δ: vcx)
     (e2: exp) (e3: exp):
-    steps (exp.if_ (exp.pure val.false) e2 e3) e3
+    steps Δ (exp.if_ (exp.pure val.false) e2 e3) e3
